restore MutableBtree

lib/DataStructures/MutableBtree.i.dfy
@@ -1,12 +1,19 @@
 include "../Lang/NativeTypes.s.dfy"
 include "../Base/NativeArrays.s.dfy"
+include "../Base/total_order.i.dfy"
+include "../Base/sequences.i.dfy"
 include "../Base/Arrays.i.dfy"
+include "../Base/Maps.s.dfy"
 include "../Base/Option.s.dfy"
+include "../Base/mathematics.i.dfy"
 include "BtreeModel.i.dfy"
 include "../../lib/Math/LinearCongruentialGenerator.s.dfy"
 
 abstract module MutableBtree {
+  import opened LinearSequence_s
+  import opened LinearSequence_i
   import opened NativeTypes
+  import opened NativeArrays
   import opened Seq = Sequences
   import opened Options
   import opened Maps
@@ -14,11 +21,12 @@ abstract module MutableBtree {
   import Arrays
   import Model : BtreeModel
 
-  export API provides WF, Interpretation, EmptyTree, Insert, Query, Empty, MinKey, MaxKey, NativeTypes, Model, Options, Maps reveals Node, NodeContents, Key, Value
+  export API provides WF, Interpretation, EmptyTree, Insert, Query, Empty, MinKey, MaxKey, NativeTypes, Model, Options, Maps reveals Node, Key, Value
   export All reveals *
     
-  type Key = Model.Key
+  type Key = Model.Keys.Element
   type Value = Model.Value
+  type Node = Model.Node
 
   function method MaxKeysPerLeaf() : uint64
     ensures 2 < MaxKeysPerLeaf() as int < Uint64UpperBound() / 4
@@ -29,1211 +37,587 @@ abstract module MutableBtree {
   function method DefaultValue() : Value
   function method DefaultKey() : Key
 
-  class Node {
-    var contents: NodeContents
-    ghost var repr: set<object>
-    ghost var height: nat
-  }
-  
-  datatype NodeContents =
-    | Leaf(nkeys: uint64, keys: array<Key>, values: array<Value>)
-    | Index(nchildren: uint64, pivots: array<Key>, children: array<Node?>)
-
-
-  function MaxSiblingHeight(nodes: seq<Node>) : int
-    ensures forall i :: 0 <= i < |nodes| ==> nodes[i].height <= MaxSiblingHeight(nodes)
-    reads Set(nodes)
-  {
-    if nodes == [] then -1
-    else Math.max(nodes[0].height, MaxSiblingHeight(nodes[1..]))
-  }
-
-  lemma MaxSiblingHeightIsSmallest(nodes: seq<Node>, parentHeight: nat)
-    ensures (forall i :: 0 <= i < |nodes| ==> nodes[i].height < parentHeight) ==>
-            MaxSiblingHeight(nodes) < parentHeight
-  {
-    var m := MaxSiblingHeight(nodes);
-    if nodes == [] {
-    } else {
-      if m == nodes[0].height {
-      } else {
-        MaxSiblingHeightIsSmallest(nodes[1..], parentHeight);
-      }
-    }
-  }
-  
-  predicate DisjointReprs(nodes: seq<Node>, i: int, j: int)
-    requires 0 <= i < |nodes|
-    requires 0 <= j < |nodes|
-    reads nodes[i], nodes[j]
-  {
-    nodes[i].repr !! nodes[j].repr
-  }
-
-  function {:opaque} SeqRepr(nodes: seq<Node>) : set<object>
-    ensures forall i :: 0 <= i < |nodes| ==> nodes[i].repr <= SeqRepr(nodes)
-    ensures nodes == [] ==> SeqRepr(nodes) == {}
-    reads Set(nodes)
-    decreases nodes
-  {
-    set i, o | 0 <= i < |nodes| && o in nodes[i].repr :: o
-  }
-
-//~  lemma SeqReprUnion(left: seq<Node>, right: seq<Node>)
-//~    ensures SeqRepr(left + right) == SeqRepr(left) + SeqRepr(right)
-//~  {
-//~    reveal_SeqRepr();
-//~    forall o | o in SeqRepr(left + right)
-//~      ensures o in SeqRepr(left) + SeqRepr(right)
-//~    {
-//~    }
-//~    forall o | o in SeqRepr(left) + SeqRepr(right)
-//~      ensures o in SeqRepr(left + right)
-//~    {
-//~      if o in SeqRepr(left) {
-//~        var i :| 0 <= i < |left| && o in left[i].repr;
-//~        assert o in (left + right)[i].repr;
-//~      } else {
-//~        var i :| 0 <= i < |right| && o in right[i].repr;
-//~        assert o in (left + right)[|left| + i].repr;
-//~      }
-//~    }
-//~  }
-  
-  lemma SeqReprSubsetExtensionality(nodes: seq<Node>, parentRepr: set<object>)
-    requires forall i :: 0 <= i < |nodes| ==> nodes[i].repr <= parentRepr
-    ensures SeqRepr(nodes) <= parentRepr
-  {
-    reveal_SeqRepr();
-  }
-
-//~  lemma SeqReprDelegation(nodes: seq<Node>, o: object) returns (idx: nat)
-//~    requires o in SeqRepr(nodes)
-//~    ensures 0 <= idx < |nodes|
-//~    ensures o in nodes[idx].repr
-//~  {
-//~    reveal_SeqRepr();
-//~    idx :| 0 <= idx < |nodes| && o in nodes[idx].repr;
-//~  }
-
-//~  lemma SubSeqRepr(nodes: seq<Node>, from: nat, to: nat)
-//~    requires 0 <= from <= to <= |nodes|
-//~    ensures SeqRepr(nodes[from..to]) <= SeqRepr(nodes)
-//~  {
-//~    reveal_SeqRepr();
-//~  }
-  
-  lemma DisjointSubSeqReprsAreDisjoint(nodes: seq<Node>, lo1: int, hi1: int, lo2: int, hi2: int)
-    requires 0 <= lo1 <= hi1 <= lo2 <= hi2 <= |nodes|
-    requires forall i, j :: 0 <= i < j < |nodes| ==> DisjointReprs(nodes, i, j)
-    ensures SeqRepr(nodes[lo1..hi1]) !! SeqRepr(nodes[lo2..hi2])
-  {
-    reveal_SeqRepr();
-    var s1 := SeqRepr(nodes[lo1..hi1]);
-    var s2 := SeqRepr(nodes[lo2..hi2]);
-    if o :| o in s1 && o in s2 {
-      var i1 :| lo1 <= i1 < hi1 && o in nodes[i1].repr;
-      var i2 :| lo2 <= i2 < hi2 && o in nodes[i2].repr;
-      assert !DisjointReprs(nodes, i1, i2);
-    }
-  }
-
-  predicate WFShapeSiblings(nodes: seq<Node>)
-    reads Set(nodes), SeqRepr(nodes)
-    decreases MaxSiblingHeight(nodes) + 1, 0
-  {
-    && (forall i :: 0 <= i < |nodes| ==> WFShape(nodes[i]))
-    && (forall i, j :: 0 <= i < j < |nodes| as int ==> DisjointReprs(nodes, i, j))
-  }
-  
-  predicate WFShapeChildren(nodes: seq<Node>, parentRepr: set<object>, parentHeight: nat)
-    reads parentRepr
-    decreases parentHeight, 1
-  {
-    MaxSiblingHeightIsSmallest(nodes, parentHeight);
-    && Set(nodes) <= parentRepr
-    && SeqRepr(nodes) <= parentRepr
-    && (forall i :: 0 <= i < |nodes| ==> nodes[i].height < parentHeight)
-    && WFShapeSiblings(nodes)
-  }
-
-  predicate WFShape(node: Node)
-    reads node, node.repr
-    decreases node.height, 2
-  {
-    if node.contents.Leaf? then
-      && node.repr == { node, node.contents.keys, node.contents.values }
-      //&& node.contents.keys != node.contents.values
-      && !Arrays.Aliases(node.contents.keys, node.contents.values)
-      && node.height == 0
-      && 0 <= node.contents.nkeys as int <= MaxKeysPerLeaf() as int == node.contents.keys.Length
-      && node.contents.values.Length == node.contents.keys.Length
-    else
-      && var nchildren := node.contents.nchildren;
-      && var children := node.contents.children;
-      && { node, node.contents.pivots, children } <= node.repr
-      && 0 < nchildren as int <= MaxChildren() as int == children.Length
-      && node.contents.pivots.Length == MaxChildren() as int - 1
-      && (forall i :: 0 <= i < nchildren ==> children[i] != null)
-      && WFShapeChildren(children[..nchildren], node.repr, node.height)
-      && (forall i :: 0 <= i < nchildren ==> node !in children[i].repr)
-      && (forall i :: 0 <= i < nchildren ==> node.contents.pivots !in children[i].repr)
-      && assert forall i :: 0 <= i < nchildren ==> children[i] == children[..nchildren][i];
-      && (forall i :: 0 <= i < nchildren ==> children !in children[i].repr)
-  }
-
-//~  lemma SeqReprSet(nodes: seq<Node>)
-//~    requires WFShapeSiblings(nodes)
-//~    ensures Set(nodes) <= SeqRepr(nodes)
-//~  {
-//~    reveal_SeqRepr();
-//~  }
-  
-  function IChildren(nodes: seq<Node>, parentheight: int) : (result: seq<Model.Node>)
-    requires forall i :: 0 <= i < |nodes| ==> WFShape(nodes[i])
-    requires forall i :: 0 <= i < |nodes| ==> nodes[i].height < parentheight
-    ensures |result| == |nodes|
-    ensures forall i :: 0 <= i < |result| ==> result[i] == I(nodes[i])
-    reads set i | 0 <= i < |nodes| :: nodes[i]
-    reads set i, o | 0 <= i < |nodes| && o in nodes[i].repr :: o
-    decreases parentheight, |nodes|
-  {
-    if |nodes| == 0 then []
-    else IChildren(DropLast(nodes), parentheight) + [I(Last(nodes))]
-  }
-  
-  function {:opaque} I(node: Node) : (result: Model.Node)
-    requires WFShape(node)
-    ensures node.contents.Leaf? <==> I(node).Leaf?
-    ensures node.contents.Leaf? ==> I(node).keys == node.contents.keys[..node.contents.nkeys]
-    ensures node.contents.Leaf? ==> I(node).values == node.contents.values[..node.contents.nkeys]
-    ensures node.contents.Index? ==> I(node).pivots == node.contents.pivots[..node.contents.nchildren-1]
-    ensures node.contents.Index? ==> |I(node).children| == node.contents.nchildren as int
-    reads node, node.repr
-    decreases node.height
-  {
-    match node.contents {
-      case Leaf(nkeys, keys, values) => Model.Leaf(keys[..nkeys], values[..nkeys])
-      case Index(nchildren, pivots, children) =>
-        assert WFShapeChildren(children[..nchildren], node.repr, node.height);
-        var bschildren := IChildren(children[..nchildren], node.height);
-        Model.Index(pivots[..nchildren-1], bschildren)
-    }
-  }
-
-  lemma IOfChild(node: Node, childidx: int)
-    requires WFShape(node)
-    requires node.contents.Index?
-    requires 0 <= childidx < node.contents.nchildren as int
-    ensures node.contents.children[childidx] != null
-    ensures WFShape(node.contents.children[childidx])
-    ensures I(node).children[childidx] == I(node.contents.children[childidx])
-  {
-    assert WFShapeSiblings(node.contents.children[..node.contents.nchildren]);
-    reveal_I();
-  }
-
-  function ISiblings(nodes: seq<Node>) : (result: seq<Model.Node>)
-    requires forall i :: 0 <= i < |nodes| ==> WFShape(nodes[i])
-    ensures |result| == |nodes|
-    ensures forall i :: 0 <= i < |result| ==> result[i] == I(nodes[i])
-    reads set i | 0 <= i < |nodes| :: nodes[i]
-    reads set i, o | 0 <= i < |nodes| && o in nodes[i].repr :: o
-  {
-    IChildren(nodes, MaxSiblingHeight(nodes) + 1)
-  }
-  
+  // TODO(jonh): A renaming, since now Node == Model.Node. Do it with sed later.
   predicate WF(node: Node)
-    ensures WF(node) ==> node in node.repr
-    reads node, node.repr
+    decreases node
   {
-    && WFShape(node)
-    && Model.WF(I(node))
+    && Model.WF(node) // TODO(jonh) things are a little ackermanny with a recursion in both Model.WF and this WF
+    && (node.Index? ==> (
+      && 0 < |node.children| <= MaxChildren() as int
+      // Recurse on children
+      && (forall i :: 0 <= i < |node.children| ==> WF(node.children[i]))
+      && lseq_has_all(node.children)
+    ))
+    && (node.Leaf? ==> (
+      && 0 <= |node.keys| <= MaxKeysPerLeaf() as int
+    ))
   }
 
+  // TODO(jonh): A renaming, since now Node == Model.Node. Do it with sed later.
   function Interpretation(node: Node) : map<Key, Value>
     requires WF(node)
-    reads node.repr
   {
-    Model.Interpretation(I(node))
+    assert Model.WF(node);
+    Model.Interpretation(node)
   }
 
-  function ToSeq(node: Node) : (kvlists: (seq<Key>, seq<Value>))
-    requires WF(node)
-    reads node.repr
+  method Route(shared keys: seq<Key>, needle: Key) returns (posplus1: uint64)
+    requires |keys| < Uint64UpperBound() / 4;
+    requires Model.Keys.IsSorted(keys)
+    ensures posplus1 as int == Model.Keys.LargestLte(keys, needle) + 1
   {
-    Model.ToSeq(I(node))
+    var pos: int64 := Model.KeysImpl.ComputeLargestLteShared(keys, needle);
+    posplus1 := (pos + 1) as uint64;
   }
-  
-  method QueryLeaf(node: Node, needle: Key) returns (result: Option<Value>)
+
+  method QueryLeaf(shared node: Node, needle: Key) returns (result: Option<Value>)
     requires WF(node)
-    requires node.contents.Leaf?
+    requires node.Leaf?
     ensures result == MapLookupOption(Interpretation(node), needle)
-    decreases node.repr, 0
   {
-    reveal_I();
     Model.reveal_Interpretation();
-    var posplus1: uint64 := Model.KeysImpl.ArrayLargestLtePlus1(node.contents.keys, 0, node.contents.nkeys, needle);
-    if 1 <= posplus1 && node.contents.keys[posplus1-1] == needle {
-      result := Some(node.contents.values[posplus1-1]);
+    assert Model.Keys.IsStrictlySorted(node.keys);
+    assert Model.Keys.IsSorted(node.keys);
+    var posplus1 := Route(node.keys, needle);
+    if 1 <= posplus1 && seq_get(node.keys, posplus1-1) == needle {
+      result := Some(seq_get(node.values, posplus1-1));
     } else {
       result := None;
     }
   }
 
-  method QueryIndex(node: Node, needle: Key) returns (result: Option<Value>)
+  method QueryIndex(shared node: Node, needle: Key) returns (result: Option<Value>)
     requires WF(node)
-    requires node.contents.Index?
+    requires node.Index?
     ensures result == MapLookupOption(Interpretation(node), needle)
-    decreases node.repr, 0
+    decreases node, 0
   {
-    reveal_I();
     Model.reveal_Interpretation();
     Model.reveal_AllKeys();
-    var posplus1: uint64 := Model.KeysImpl.ArrayLargestLtePlus1(node.contents.pivots, 0, node.contents.nchildren-1, needle);
-    assert WFShapeChildren(node.contents.children[..node.contents.nchildren], node.repr, node.height);
-    result := Query(node.contents.children[posplus1], needle);
+    var posplus1:uint64 := Route(node.pivots, needle);
+    result := Query(lseq_peek(node.children, posplus1), needle);
     if result.Some? {
-      Model.InterpretationDelegation(I(node), needle);
+      Model.InterpretationDelegation(node, needle);
     }
   }
 
-  method Query(node: Node, needle: Key) returns (result: Option<Value>)
+  method Query(shared node: Node, needle: Key) returns (result: Option<Value>)
     requires WF(node)
     ensures result == MapLookupOption(Interpretation(node), needle)
-    decreases node.repr, 1
+    decreases node, 1
   {
-    match node.contents {
-      case Leaf(_, _, _) => result := QueryLeaf(node, needle);
-      case Index(_, _, _) => result := QueryIndex(node, needle);
+    shared match node {
+      case Leaf(_, _) => result := QueryLeaf(node, needle);
+      case Index(_, _) => result := QueryIndex(node, needle);
     }
   }
 
-  method Empty(node: Node) returns (result: bool)
+  method Empty(shared node: Node) returns (result: bool)
     requires WF(node)
     ensures result == (|Interpretation(node)| == 0)
   {
-    if node.contents.Leaf? {
+    if node.Leaf? {
       Model.reveal_Interpretation();
-      result := 0 == node.contents.nkeys;
-      assert !result ==> node.contents.keys[0] in Interpretation(node);
+      result := 0 == seq_length(node.keys);
+      assert !result ==> node.keys[0] in Interpretation(node);
     } else {
-      Model.IndexesNonempty(I(node));
+      Model.IndexesNonempty(node);
       result := false;
     }
   }
   
-  method MinKeyInternal(node: Node) returns (result: Key)
+  method MinKeyInternal(shared node: Node) returns (result: Key)
     requires WF(node)
     requires 0 < |Interpretation(node)|
-    ensures result == Model.MinKey(I(node))
-    decreases node.repr
+    ensures result == Model.MinKey(node)
   {
-    if node.contents.Leaf? {
-      assert 0 < node.contents.nkeys by {
+    if node.Leaf? {
+      assert 0 < |node.keys| by {
         Model.reveal_Interpretation();
       }
-      assert node.contents.keys[0] == node.contents.keys[..node.contents.nkeys][0];
-      result := node.contents.keys[0];
+      assert node.keys[0] == node.keys[..|node.keys|][0];
+      result := seq_get(node.keys, 0);
     } else {
-      assert WFShapeChildren(node.contents.children[..node.contents.nchildren], node.repr, node.height);
-      IOfChild(node, 0);
-      assert WF(node.contents.children[0]);
-      Model.ChildOfIndexNonempty(I(node), 0);
-      result := MinKeyInternal(node.contents.children[0]);
+      // IOfChild(node, 0);
+      assert WF(node.children[0]);
+      Model.ChildOfIndexNonempty(node, 0);
+      result := MinKeyInternal(lseq_peek(node.children, 0));
     }
   }
 
   // We separate MinKey and MinKeyInternal in order to keep the API
   // export set clean.  (MinKeyInternal needs to mention I(), but we
   // don't want to export it.)
-  method MinKey(node: Node) returns (result: Key)
+  method MinKey(shared node: Node) returns (result: Key)
     requires WF(node)
     requires 0 < |Interpretation(node)|
     ensures result in Interpretation(node)
     ensures forall key | key in Interpretation(node) :: Model.Keys.lte(result, key)
   {
     result := MinKeyInternal(node);
-    Model.MinKeyProperties(I(node));
+    Model.MinKeyProperties(node);
   }
   
-  method MaxKeyInternal(node: Node) returns (result: Key)
+  method MaxKeyInternal(shared node: Node) returns (result: Key)
     requires WF(node)
     requires 0 < |Interpretation(node)|
-    ensures result == Model.MaxKey(I(node))
-    decreases node.repr
+    ensures result == Model.MaxKey(node)
   {
-    if node.contents.Leaf? {
-      assert 0 < node.contents.nkeys by {
+    if node.Leaf? {
+      assert 0 < |node.keys| by {
         Model.reveal_Interpretation();
       }
-      var nkeys: uint64 := node.contents.nkeys;
-      assert node.contents.keys[nkeys - 1] == node.contents.keys[..nkeys][nkeys - 1];
-      result := node.contents.keys[nkeys-1];
+      var nkeys: uint64 := seq_length(node.keys) as uint64;
+      assert node.keys[nkeys - 1] == node.keys[..nkeys][nkeys - 1];
+      result := seq_get(node.keys, nkeys-1);
     } else {
-      var nchildren: uint64 := node.contents.nchildren;
-      assert WFShapeChildren(node.contents.children[..node.contents.nchildren], node.repr, node.height);
-      IOfChild(node, nchildren as nat - 1);
-      assert WF(node.contents.children[nchildren - 1]);
-      Model.ChildOfIndexNonempty(I(node), nchildren as nat - 1);
-      result := MaxKeyInternal(node.contents.children[nchildren - 1]);
+      var nchildren: uint64 := lseq_length_uint64(node.children);
+      // IOfChild(node, nchildren as nat - 1);
+      assert WF(node.children[nchildren as nat - 1]);
+      Model.ChildOfIndexNonempty(node, nchildren as nat - 1);
+      result := MaxKeyInternal(lseq_peek(node.children, nchildren - 1));
     }
   }
   
   // We separate MaxKey and MaxKeyInternal in order to keep the API
   // export set clean.  (MaxKeyInternal needs to mention I(), but we
   // don't want to export it.)
-  method MaxKey(node: Node) returns (result: Key)
+  method MaxKey(shared node: Node) returns (result: Key)
     requires WF(node)
     requires 0 < |Interpretation(node)|
     ensures result in Interpretation(node)
     ensures forall key | key in Interpretation(node) :: Model.Keys.lte(key, result)
   {
     result := MaxKeyInternal(node);
-    Model.MaxKeyProperties(I(node));
+    Model.MaxKeyProperties(node);
   }
   
-  method EmptyTree() returns (root: Node)
+  method EmptyTree() returns (linear root: Node)
     ensures WF(root)
-    ensures fresh(root.repr)
     ensures Interpretation(root) == map[]
-    ensures root.contents.Leaf?
+    ensures root.Leaf?
   {
-    var rootkeys := newArrayFill(MaxKeysPerLeaf(), DefaultKey());
-    var rootvalues := newArrayFill(MaxKeysPerLeaf(), DefaultValue());
-    root := new Node;
-    root.contents := Leaf(0, rootkeys, rootvalues);
-    root.repr := {root, rootkeys, rootvalues};
-    root.height := 0;
+    linear var rootkeys := seq_empty();
+    linear var rootvalues := seq_empty();
+    root := Model.Leaf(rootkeys, rootvalues);
     Model.reveal_Interpretation();
-    Model.Keys.reveal_IsStrictlySorted();
   }
 
-  method LeafFromSeqs(keys: seq<Key>, values: seq<Value>)
-    returns (node: Node)
-    requires |keys| == |values| <= MaxKeysPerLeaf() as int
-    ensures WFShape(node)
-    ensures node.contents.Leaf?
-    ensures fresh(node.repr)
-    ensures node.contents.keys[..node.contents.nkeys] == keys
-    ensures node.contents.values[..node.contents.nkeys] == values
-  {
-    node := EmptyTree();
-    CopySeqIntoArray(keys, 0, node.contents.keys, 0, |keys| as uint64);
-    CopySeqIntoArray(values, 0, node.contents.values, 0, |values| as uint64);
-    node.contents := node.contents.(nkeys := |keys| as uint64);
-    assert node.contents.keys[..node.contents.nkeys] == keys;
-  }
+//  method LeafFromSeqs(keys: seq<Key>, values: seq<Value>)
+//    returns (node: Node)
+//    requires |keys| == |values| <= MaxKeysPerLeaf() as int
+//    ensures WFShape(node)
+//    ensures node.Leaf?
+//    ensures fresh(node.repr)
+//    ensures node.keys[..|node.keys|] == keys
+//    ensures node.values[..|node.keys|] == values
+//  {
+//    node := EmptyTree();
+//    CopySeqIntoArray(keys, 0, node.keys, 0, |keys| as uint64);
+//    CopySeqIntoArray(values, 0, node.values, 0, |values| as uint64);
+//    node := node.(nkeys := |keys| as uint64);
+//    assert node.keys[..|node.keys|] == keys;
+//  }
+//
+//  method IndexFromChildren(pivots: seq<Key>, children: seq<Node>, ghost height: nat) returns (node: Node)
+//    requires 0 < |children| <= MaxChildren() as int
+//    requires |pivots| == |children|-1
+//    ensures node.Index?
+//    ensures node.pivots.Length == MaxChildren() as int - 1
+//    ensures node.children.Length == MaxChildren() as int
+//    ensures |node.children| == |children| as uint64
+//    ensures node.pivots[..|node.children|-1] == pivots
+//    ensures node.children[..|node.children|] == children
+//    ensures fresh(node)
+//    ensures fresh(node.pivots)
+//    ensures fresh(node.children)
+//    ensures node.repr == {node, node.pivots, node.children} + SeqRepr(children)
+//    ensures node.height == height
+//  {
+//    var pivotarray := newArrayFill(MaxChildren()-1, DefaultKey());
+//    var childarray := newArrayFill(MaxChildren(), null);
+//    CopySeqIntoArray(pivots, 0, pivotarray, 0, |pivots| as uint64);
+//    CopySeqIntoArray(children, 0, childarray, 0, |children| as uint64);
+//    node := new Node;
+//    node := Index(|children| as uint64, pivotarray, childarray);
+//    node.repr := {node, node.pivots, node.children} + SeqRepr(children);
+//    node.height := height;
+//  }
 
-  method IndexFromChildren(pivots: seq<Key>, children: seq<Node>, ghost height: nat) returns (node: Node)
-    requires 0 < |children| <= MaxChildren() as int
-    requires |pivots| == |children|-1
-    ensures node.contents.Index?
-    ensures node.contents.pivots.Length == MaxChildren() as int - 1
-    ensures node.contents.children.Length == MaxChildren() as int
-    ensures node.contents.nchildren == |children| as uint64
-    ensures node.contents.pivots[..node.contents.nchildren-1] == pivots
-    ensures node.contents.children[..node.contents.nchildren] == children
-    ensures fresh(node)
-    ensures fresh(node.contents.pivots)
-    ensures fresh(node.contents.children)
-    ensures node.repr == {node, node.contents.pivots, node.contents.children} + SeqRepr(children)
-    ensures node.height == height
-  {
-    var pivotarray := newArrayFill(MaxChildren()-1, DefaultKey());
-    var childarray := newArrayFill(MaxChildren(), null);
-    CopySeqIntoArray(pivots, 0, pivotarray, 0, |pivots| as uint64);
-    CopySeqIntoArray(children, 0, childarray, 0, |children| as uint64);
-    node := new Node;
-    node.contents := Index(|children| as uint64, pivotarray, childarray);
-    node.repr := {node, node.contents.pivots, node.contents.children} + SeqRepr(children);
-    node.height := height;
-  }
-  
-  predicate method Full(node: Node)
-    reads node
-  {
-    match node.contents {
-      case Leaf(nkeys, _, _) => nkeys == MaxKeysPerLeaf()
-      case Index(nchildren, _, _) => nchildren == MaxChildren()
-    }
-  }
-
-  method SplitLeaf(node: Node, nleft: uint64, ghost pivot: Key) returns (right: Node)
+  predicate method Full(shared node: Node)
     requires WF(node)
-    requires node.contents.Leaf?
-    requires 0 < nleft < node.contents.nkeys
-    requires Model.Keys.lt(node.contents.keys[nleft-1], pivot)
-    requires Model.Keys.lte(pivot, node.contents.keys[nleft])
-    ensures WFShape(node)
-    ensures WFShape(right)
-    ensures node.repr == old(node.repr)
-    ensures fresh(right.repr)
-    ensures Model.SplitLeaf(old(I(node)), I(node), I(right), pivot)
-    ensures node.contents.nkeys == nleft
-    modifies node
   {
-    reveal_I();
-    Model.Keys.StrictlySortedSubsequence(node.contents.keys[..node.contents.nkeys], nleft as int, node.contents.nkeys as int);
-    assert node.contents.keys[nleft..node.contents.nkeys] == node.contents.keys[..node.contents.nkeys][nleft..node.contents.nkeys];
-    right := LeafFromSeqs(node.contents.keys[nleft..node.contents.nkeys], node.contents.values[nleft..node.contents.nkeys]);
-
-    node.contents := Leaf(nleft, node.contents.keys, node.contents.values);
-    Model.Keys.IsStrictlySortedImpliesLt(old(node.contents.keys[..node.contents.nkeys]), nleft as int - 1, nleft as int);
-  }
-
-  predicate ObjectIsInSubtree(node: Node, o: object, i: int)
-    requires WFShape(node)
-    requires node.contents.Index?
-    requires 0 <= i < node.contents.nchildren as int
-    reads node.repr
-  {
-    assert WFShapeChildren(node.contents.children[..node.contents.nchildren], node.repr, node.height);
-    o in node.contents.children[i].repr
-  }
-
-  function SubRepr(node: Node, from: int, to: int) : (result: set<object>)
-    requires WFShape(node)
-    requires node.contents.Index?
-    requires 0 <= from <= to <= node.contents.nchildren as int
-    reads node.repr
-  {
-    assert WFShapeChildren(node.contents.children[..node.contents.nchildren], node.repr, node.height);
-    assert forall i :: from <= i < to ==> node.contents.children[i] != null;
-    assert forall i :: from <= i < to ==> node.contents.children[i] in node.repr;
-    SeqRepr(node.contents.children[from..to])
-  }
-
-  predicate DisjointSubtrees(contents: NodeContents, i: int, j: int)
-    requires contents.Index?
-    requires 0 <= i < contents.nchildren as int
-    requires 0 <= j < contents.nchildren as int
-    requires contents.nchildren as int <= contents.children.Length
-    requires forall l :: 0 <= l < contents.nchildren ==> contents.children[l] != null
-    requires contents.children[j] != null
-    reads contents.children, contents.children[i], contents.children[j]
-  {
-    DisjointReprs(contents.children[..contents.nchildren], i, j)
-  }
-  
-  lemma SubReprsDisjoint(node: Node, from1: int, to1: int, from2: int, to2: int)
-    requires WFShape(node)
-    requires node.contents.Index?
-    requires 0 <= from1 <= to1 <= from2 <= to2 <= node.contents.nchildren as int
-    ensures SubRepr(node, from1, to1) !! SubRepr(node, from2, to2)
-  {
-    assert node.contents.children[..node.contents.nchildren][from1..to1]
-      == node.contents.children[from1..to1];
-    assert node.contents.children[..node.contents.nchildren][from2..to2]
-      == node.contents.children[from2..to2];
-    assert WFShapeSiblings(node.contents.children[..node.contents.nchildren]);
-    // assert forall i, j :: 0 <= i < j < node.contents.nchildren ==>
-    //     DisjointReprs(node.contents.children[..node.contents.nchildren], i as int, j as int);
-    DisjointSubSeqReprsAreDisjoint(node.contents.children[..node.contents.nchildren], from1, to1, from2, to2);
-  }
-
-  lemma SubReprUpperBound(node: Node, from: int, to: int)
-    requires WFShape(node)
-    requires node.contents.Index?
-    requires 1 < node.contents.nchildren
-    requires 0 <= from <= to <= node.contents.nchildren as int
-    ensures SubRepr(node, from, to) <= node.repr - {node, node.contents.pivots, node.contents.children}
-    ensures to - from < node.contents.nchildren as int ==> SubRepr(node, from, to) < node.repr - {node, node.contents.pivots, node.contents.children}
-  {
-    reveal_SeqRepr();
-    
-    var subrepr := SubRepr(node, from, to);
-    var nchildren := node.contents.nchildren;
-    var pivots := node.contents.pivots;
-    var children := node.contents.children;
-
-    forall o | o in subrepr
-      ensures o in node.repr
-    {
-      var i :| from <= i < to && o in node.contents.children[i].repr;
-    }
-    assert subrepr <= node.repr;
-    assert pivots !in subrepr;
-    assert children !in subrepr;
-    assert subrepr <= node.repr - {node, pivots, children};
-    
-    if to - from < nchildren as int {
-      assert WFShapeChildren(node.contents.children[..node.contents.nchildren], node.repr, node.height);
-      assert WFShape(children[0]);
-      assert WFShape(children[nchildren-1]);
-      assert children[0].repr < node.repr;
-      assert children[0].repr != {};
-      assert children[nchildren-1].repr < node.repr;
-      assert children[nchildren-1].repr != {};
-      if 0 < from {
-        forall o | o in subrepr
-          ensures o !in children[0].repr
-        {
-          if o == pivots {
-          } else if o == children {
-          } else {
-            var i :| from <= i < to && o in node.repr && o in node.contents.children[i].repr; 
-            assert DisjointSubtrees(node.contents, 0, i);
-          }
-        }
-        assert subrepr < node.repr - {node, pivots, children};
-      } else {
-        assert to < nchildren as int;
-        forall o | o in subrepr
-          ensures o !in children[nchildren - 1].repr
-        {
-          if o == pivots {
-          } else if o == children {
-          } else {
-            var i :| from <= i < to && o in node.repr && o in node.contents.children[i].repr; 
-            assert DisjointSubtrees(node.contents, i, nchildren as int - 1);
-          }
-        }
-        var wit :| wit in children[nchildren-1].repr;
-        assert wit !in subrepr;
-        assert subrepr < node.repr - {node, pivots, children};
-      }
+    shared match node {
+      case Leaf(keys, _) => seq_length(keys) == MaxKeysPerLeaf()
+      case Index(_, children) => lseq_length_uint64(children) == MaxChildren()
     }
   }
 
-  lemma SubReprLowerBound(node: Node, from: int, to: int)
-    requires WFShape(node)
-    requires node.contents.Index?
-    requires 1 <= node.contents.nchildren
-    requires 0 <= from <= to <= node.contents.nchildren as int
-    ensures forall i :: from <= i < to ==> node.contents.children[i] != null
-    ensures forall i :: from <= i < to ==> node.contents.children[i].repr <= SubRepr(node, from, to)
-  {
-    reveal_SeqRepr();
-    
-    var subrepr := SubRepr(node, from, to);
-    var nchildren := node.contents.nchildren;
-    var pivots := node.contents.pivots;
-    var children := node.contents.children;
-    
-    forall o | o in subrepr
-      ensures o in node.repr
-    {
-      var i :| from <= i < to && o in node.contents.children[i].repr;
-    }
-    assert subrepr <= node.repr;
-    assert pivots !in subrepr;
-    assert children !in subrepr;
-    assert subrepr <= node.repr - {node, pivots, children};
-    
-    forall i | from <= i < to
-      ensures children[i].repr <= subrepr
-    {
-      forall o | o in children[i].repr
-        ensures o in subrepr
-      {
-        //assert ObjectIsInSubtree(node, o, i);
-      }
-    }
-  }
+  // TODO(robj): someday, if perf demands it: switch to a linear version of
+  // MutableVec as the underlying storage to save some sequence copies?
 
-  
-  method IndexPrefix(node: Node, newnchildren: uint64)
+  method SplitLeaf(linear node: Node, nleft: uint64, ghost pivot: Key)
+    returns (linear left: Node, linear right: Node)
     requires WF(node)
-    requires node.contents.Index?
-    requires 1 <= newnchildren
-    requires 0 <= newnchildren <= node.contents.nchildren
-    ensures WFShape(node)
-    ensures node.repr == old({node, node.contents.pivots, node.contents.children} + SubRepr(node, 0, newnchildren as int))
-    ensures node.height == old(node.height)
-    ensures I(node) == Model.SubIndex(old(I(node)), 0, newnchildren as int)
-    modifies node
+    requires node.Leaf?
+    requires 0 < nleft as int < |node.keys|
+    requires Model.Keys.lt(node.keys[nleft-1], pivot)
+    requires Model.Keys.lte(pivot, node.keys[nleft])
+    ensures WF(left)
+    ensures WF(right)
+    ensures Model.SplitLeaf(node, left, right, pivot)
+    ensures |left.keys| == nleft as int
   {
-    assert WFShapeChildren(node.contents.children[..node.contents.nchildren], node.repr, node.height);
-    ghost var oldinode := I(node);
-    SubReprLowerBound(node, 0, newnchildren as int);
+    ghost var nkeys := |node.keys|;
+    Model.Keys.StrictlySortedSubsequence(node.keys, nleft as int, nkeys);
+    Model.Keys.StrictlySortedSubsequence(node.keys, 0, nleft as int);
+    Model.Keys.IsStrictlySortedImpliesLt(node.keys, nleft as int - 1, nleft as int);
+    assert node.keys[nleft..nkeys] == node.keys[..nkeys][nleft..nkeys];
 
-    node.repr := {node, node.contents.pivots, node.contents.children} + SubRepr(node, 0, newnchildren as int);
-    node.contents := node.contents.(nchildren := newnchildren);
+    var nright:uint64 := seq_length(node.keys) as uint64 - nleft;
+    linear var Leaf(keys, values) := node;
 
-    ghost var newchildren := node.contents.children[..newnchildren];
-    assert forall i :: 0 <= i < newnchildren ==> WFShape(newchildren[i]);
-    assert newchildren == old(node.contents.children[..node.contents.nchildren])[..newnchildren];
-    forall i, j | 0 <= i < j < |newchildren|
-      ensures DisjointReprs(newchildren, i, j)
-    {
-      assert old(DisjointReprs(node.contents.children[..node.contents.nchildren], i, j));
-    }
-    assert WFShape(node);
-    ghost var newinode := I(node);
-    reveal_I();
-    assert newinode == Model.SubIndex(oldinode, 0, newnchildren as int);
+    // TODO(robj): perf-pportunity: recycle node as left, rather than copy-and-free.
+    linear var leftKeys := AllocAndCopy(keys, 0, nleft);
+    linear var rightKeys := AllocAndCopy(keys, nleft, nleft + nright);
+    linear var leftValues := AllocAndCopy(values, 0, nleft);
+    linear var rightValues := AllocAndCopy(values, nleft, nleft + nright);
+    left := Model.Leaf(leftKeys, leftValues);
+    right := Model.Leaf(rightKeys, rightValues);
+    var _ := seq_free(keys);
+    var _ := seq_free(values);
   }
 
-  method SubIndex(node: Node, from: uint64, to: uint64) returns (subnode: Node)
+  // We need to measure the height of Nodes to manage termination in the mutual
+  // recursion between InsertNode and InsertIndex. You'd think that we wouldn't
+  // need to, since datatypes are well-founded. But when we SplitChildOfIndex,
+  // we replace some children with other children. The new children are of no
+  // greater height, but they don't order in Dafny's internal datatype lattice.
+  // Hence this machinery for explicitly measuring height.
+  function IndexHeights(node: Node): seq<int>
+    requires Model.WF(node)
+    requires node.Index?
+    decreases node, 0
+  {
+      seq(|node.children|, i requires 0<=i<|node.children| => Height(node.children[i]))
+  }
+
+  function {:opaque} Height(node: Node): nat
+    requires Model.WF(node)
+    ensures node.Leaf? ==> Height(node) == 0
+    decreases node, 1
+  {
+    if node.Leaf?
+    then 0
+    else
+      var heights := IndexHeights(node); seqMax(heights) + 1
+  }
+
+  lemma SubIndexHeight(node: Node, from: nat, to: nat)
+    requires Model.WF(node)
+    requires node.Index?
+    requires 0 <= from < to <= |node.children|
+    ensures Model.WF(Model.SubIndex(node, from, to))
+    ensures Height(Model.SubIndex(node, from, to)) <= Height(node)
+  {
+    Model.SubIndexPreservesWF(node, from, to);
+    var heights := IndexHeights(node);
+    reveal_Height();
+    assert IndexHeights(Model.SubIndex(node, from, to)) == heights[from .. to]; // trigger
+    SubseqMax(heights, from, to);
+  }
+
+  method SplitIndex(linear node: Node, nleft: uint64)
+    returns (linear left: Node, linear right: Node, pivot: Key)
     requires WF(node)
-    requires node.contents.Index?
-    requires 1 < node.contents.nchildren
-    requires 0 <= from < to <= node.contents.nchildren
-    ensures WFShape(subnode)
-    ensures subnode.contents.Index?
-    ensures subnode.repr == SubRepr(node, from as int, to as int) + {subnode, subnode.contents.pivots, subnode.contents.children}
-    ensures subnode.height == node.height
-    ensures I(subnode) == Model.SubIndex(I(node), from as int, to as int)
-    ensures fresh(subnode)
-    ensures fresh(subnode.contents.pivots)
-    ensures fresh(subnode.contents.children)
+    requires node.Index?
+    requires 2 <= |node.children|
+    requires 0 < nleft as nat < |node.children|
+    ensures WF(left)
+    ensures WF(right)
+    ensures Model.SplitIndex(node, left, right, pivot)
+    ensures |left.children| == nleft as nat
+    ensures pivot == node.pivots[nleft-1]
+    ensures Height(left) <= Height(node)
+    ensures Height(right) <= Height(node)
   {
-    assert WFShapeChildren(node.contents.children[..node.contents.nchildren], node.repr, node.height);
+    assert nleft as nat < |node.children| == lseq_length_uint64(node.children) as nat;
+    var nright:uint64 := lseq_length_uint64(node.children) - nleft;
+    linear var Index(pivots, children) := node;
+    pivot := seq_get(pivots, nleft-1);
 
-    subnode := IndexFromChildren(node.contents.pivots[from..to-1], node.contents.children[from..to], node.height);
+    // TODO(robj): perf-pportunity: recycle node as left, rather than copy-and-free.
+    assert 0 <= nleft - 1;
+    linear var leftPivots := AllocAndCopy(pivots, 0, nleft-1);
+    linear var rightPivots := AllocAndCopy(pivots, nleft, nleft + nright - 1);
 
-    ghost var newchildren := subnode.contents.children[..subnode.contents.nchildren];
-    assert forall i :: 0 <= i < |newchildren| ==> WFShape(newchildren[i]);
-    forall i, j | 0 <= i < j < |newchildren|
-      ensures DisjointReprs(newchildren, i, j)
-    {
-      assert DisjointSubtrees(node.contents, from as int + i, from as int + j);
-    }
-    forall i | 0 <= i < |newchildren|
-      ensures subnode !in newchildren[i].repr
-    {
-    }
-    assert WFShapeSiblings(newchildren);
-    assert WFShapeChildren(newchildren, subnode.repr, subnode.height);
+    linear var leftChildren, rightChildren;
+    children, leftChildren := AllocAndMoveLseq(children, 0, nleft);
+    children, rightChildren := AllocAndMoveLseq(children, nleft, nleft + nright);
+    left := Model.Index(leftPivots, leftChildren);
+    right := Model.Index(rightPivots, rightChildren);
 
-    reveal_I();
-    assert node.contents.pivots[from..to-1] == I(node).pivots[from..to-1];
+    ImagineInverse(left.children);
+    assert lseqs(right.children) == lseqs(node.children)[|left.children|..|node.children|];  // observe trigger
+    ImagineInverse(right.children);
+
+    assert Model.AllKeysBelowBound(node, nleft as int - 1); // trigger
+    assert Model.AllKeysAboveBound(node, nleft as int); // trigger
+    Model.SplitIndexPreservesWF(node, left, right, pivot);
+    var _ := seq_free(pivots);
+    lseq_free(children);
+    SubIndexHeight(node, 0, nleft as nat);
+    SubIndexHeight(node, nleft as nat, nleft as nat + nright as nat);
   }
 
-  method SplitIndex(node: Node, nleft: uint64) returns (right: Node, pivot: Key)
-    requires WF(node)
-    requires node.contents.Index?
-    requires 2 <= node.contents.nchildren
-    requires 0 < nleft < node.contents.nchildren
-    ensures WFShape(node)
-    ensures WFShape(right)
-    ensures node.repr <= old(node.repr)
-    ensures node.repr !! right.repr
-    ensures fresh(right.repr - old(node.repr))
-    ensures node.height == old(node.height) == right.height
-    ensures Model.SplitIndex(old(I(node)), I(node), I(right), pivot)
-    ensures node.contents.nchildren == nleft
-    ensures pivot == old(node.contents.pivots[nleft-1])
-    modifies node
-  {
-    SubReprsDisjoint(node, 0, nleft as int, nleft as int, node.contents.nchildren as int);
-    SubReprUpperBound(node, 0, nleft as int);
-    SubReprUpperBound(node, nleft as int, node.contents.nchildren as int);
-    assert Model.AllKeysBelowBound(I(node), nleft as int - 1);
-    assert Model.AllKeysAboveBound(I(node), nleft as int);
-    right := SubIndex(node, nleft, node.contents.nchildren);
-    pivot := node.contents.pivots[nleft-1];
-    IOfChild(node, 0);
-    IndexPrefix(node, nleft);
-    ghost var inode := old(I(node));
-    ghost var iright := I(right);
-    assert Model.AllKeysBelowBound(inode, 0);
-    assert iright.children[0] == inode.children[nleft];
-    Model.Keys.IsStrictlySortedImpliesLte(old(I(node)).pivots, 0, (nleft - 1) as int);
-    reveal_I();
-  }
-
-  method SplitNode(node: Node) returns (right: Node, pivot: Key)
+  method SplitNode(linear node: Node) returns (linear left: Node, linear right: Node, pivot: Key)
     requires WF(node)
     requires Full(node)
-    ensures WFShape(node)
-    ensures WFShape(right)
-    ensures node.height == old(node.height)
-    ensures right.height == old(node.height)
-    ensures node.repr <= old(node.repr)
-    ensures fresh(right.repr - old(node.repr))
-    ensures node.repr !! right.repr
-    ensures !Full(node)
+    ensures WF(left)
+    ensures WF(right)
+    ensures !Full(left)
     ensures !Full(right)
-    ensures Model.SplitNode(old(I(node)), I(node), I(right), pivot)
-    ensures pivot in Model.AllKeys(old(I(node)))
-    modifies node
+    ensures Model.SplitNode(node, left, right, pivot)
+    ensures pivot in Model.AllKeys(node)
+    ensures Height(left) <= Height(node)
+    ensures Height(right) <= Height(node)
   {
-    if node.contents.Leaf? {
-      var boundary := node.contents.nkeys/2;
-      pivot := node.contents.keys[boundary];
-      Model.Keys.IsStrictlySortedImpliesLt(node.contents.keys[..node.contents.nkeys], boundary as int - 1, boundary as int);
-      right := SplitLeaf(node, node.contents.nkeys / 2, pivot);
+    if node.Leaf? {
+      var boundary := seq_length(node.keys) / 2;
+      pivot := seq_get(node.keys, boundary);
+      Model.Keys.IsStrictlySortedImpliesLt(node.keys, boundary as int - 1, boundary as int);
+      left, right := SplitLeaf(node, boundary, pivot);
     } else {
-      var boundary := node.contents.nchildren/2;
-      right, pivot := SplitIndex(node, boundary);
+      var boundary := lseq_length_uint64(node.children) / 2;
+//      assert 2 <= |node.children|;
+//      assert 0 < boundary as nat < |node.children|;
+      left, right, pivot := SplitIndex(node, boundary);
     }
     Model.reveal_AllKeys();
+//    assert !Full(left);
+//    assert !Full(right);
   }
 
-  // twostate lemma SplitChildOfIndexPreservesDisjointSubtrees(node: Node, childidx: int)
-  //   requires old(WFShape(node))
-  //   requires old(node.contents).Index?
-  //   requires old(!Full(node))
-  //   requires 0 <= childidx < old(node.contents).nchildren as int
-  //   requires node.contents.Index?
-  //   requires node.contents.nchildren == old(node.contents).nchildren + 1
-  //   requires node.contents.children.Length == old(node.contents.children.Length)
-  //   requires forall i :: 0 <= i < node.contents.nchildren ==> node.contents.children[i] != null
-  //   requires forall i :: 0 <= i < childidx ==> node.contents.children[i].repr == old(node.contents.children[i].repr)
-  //   requires node.contents.children[childidx].repr <= old(node.contents.children[childidx].repr)
-  //   requires fresh(node.contents.children[childidx+1].repr - old(node.contents.children[childidx].repr))
-  //   requires forall i :: childidx+1 < i < node.contents.nchildren as int ==> node.contents.children[i].repr == old(node.contents.children[i-1].repr)
-  //   requires DisjointSubtrees(node.contents, childidx, (childidx + 1));
-  //   ensures forall i, j :: 0 <= i < j < node.contents.nchildren ==> DisjointSubtrees(node.contents, i as int, j as int)
-  // {
-  //   forall i, j | 0 <= i < j < node.contents.nchildren as int
-  //     ensures DisjointSubtrees(node.contents, i, j)
-  //   {
-  //     if                           j <  childidx       {
-  //       assert old(DisjointSubtrees(node.contents, i, j));
-  //     } else if                    j == childidx       {
-  //       assert old(DisjointSubtrees(node.contents, i, j));
-  //     } else if i < childidx     && j == childidx+1     {
-  //       assert old(DisjointSubtrees(node.contents, i, j - 1));
-  //     } else if i == childidx    && j == childidx+1     {
-  //       assert DisjointSubtrees(node.contents, childidx, (childidx + 1));
-  //     } else if i < childidx     &&      childidx+1 < j {
-  //       assert old(DisjointSubtrees(node.contents, i, (j-1)));
-  //     } else if i == childidx    &&      childidx+1 < j {
-  //       assert old(DisjointSubtrees(node.contents, i, (j-1)));
-  //     } else if i == childidx+1  &&      childidx+1 < j {
-  //       assert old(DisjointSubtrees(node.contents, (i-1), (j-1)));
-  //     } else {
-  //       assert old(DisjointSubtrees(node.contents, (i-1), (j-1)));
-  //     }
-  //   }
-  // }
-
-  twostate lemma SplitChildOfIndexPreservesWFShape(node: Node, childidx: int)
-    requires old(WFShape(node))
-    requires old(node.contents).Index?
-    requires old(!Full(node))
-    requires 0 <= childidx < old(node.contents).nchildren as int
-    requires node.contents.Index?
-    requires node.contents.nchildren == old(node.contents).nchildren + 1
-    requires node.contents.children == old(node.contents.children)
-    requires node.contents.pivots == old(node.contents.pivots)
-    requires node.height == old(node.height)
-    requires unchanged(old(node.repr) - {node, node.contents.pivots, node.contents.children, node.contents.children[childidx]})
-    requires forall i :: 0 <= i < childidx ==> node.contents.children[i] == old(node.contents.children[i])
-    requires forall i :: childidx + 1 < i < node.contents.nchildren as int ==> node.contents.children[i] == old(node.contents.children[i-1])
-    requires old(node.contents.children[childidx]) != null
-    requires node.contents.children[childidx] != null
-    requires WFShape(node.contents.children[childidx])
-    requires node.contents.children[childidx].repr <= old(node.contents.children[childidx].repr)
-    requires node.contents.children[childidx].height == old(node.contents.children[childidx].height)
-    requires node.contents.children[childidx+1] != null
-    requires WFShape(node.contents.children[childidx+1])
-    requires fresh(node.contents.children[childidx+1].repr - old(node.contents.children[childidx].repr))
-    requires node.contents.children[childidx+1].height == old(node.contents.children[childidx].height)
-    requires DisjointSubtrees(node.contents, childidx, (childidx + 1))
-    requires node.repr == old(node.repr) + node.contents.children[childidx+1].repr
-    ensures WFShape(node)
-  {
-    assert old(WFShapeChildren(node.contents.children[..node.contents.nchildren], node.repr, node.height));
-
-    var newchildren := node.contents.children[..node.contents.nchildren];
-    
-    forall i | 0 <= i < node.contents.nchildren as int
-      ensures newchildren[i] != null
-      ensures newchildren[i] in node.repr
-      ensures newchildren[i].repr < node.repr
-      ensures node !in newchildren[i].repr
-      ensures node.contents.pivots !in newchildren[i].repr
-      ensures node.contents.children !in newchildren[i].repr
-      ensures newchildren[i].height < node.height
-      ensures WFShape(newchildren[i])
-    {
-      if i < childidx {
-        assert old(DisjointSubtrees(node.contents, i, childidx));
-      } else if i == childidx {
-      } else if i == childidx + 1 {
-      } else {
-        assert old(DisjointSubtrees(node.contents, childidx, i-1));
-      }
-    }
-    SeqReprSubsetExtensionality(newchildren, node.repr);
-      
-    forall i, j | 0 <= i < j < node.contents.nchildren as int
-      ensures DisjointReprs(newchildren, i, j)
-    {
-      if                           j <  childidx       {
-        assert old(DisjointSubtrees(node.contents, i, childidx));
-        assert old(DisjointSubtrees(node.contents, j, childidx));
-        assert old(DisjointSubtrees(node.contents, i, j));
-        assert old(WFShape(node.contents.children[i]));
-        assert old(WFShape(node.contents.children[j]));
-      } else if                    j == childidx       {
-        assert old(DisjointSubtrees(node.contents, i, childidx));
-        assert old(DisjointSubtrees(node.contents, i, j));
-        assert old(WFShape(node.contents.children[i]));
-      } else if i < childidx     && j == childidx+1     {
-        assert old(DisjointSubtrees(node.contents, i, childidx));
-        assert old(DisjointSubtrees(node.contents, i, j - 1));
-        assert old(WFShape(node.contents.children[i]));
-      } else if i == childidx    && j == childidx+1     {
-      } else if i < childidx     &&      childidx+1 < j {
-        assert old(DisjointSubtrees(node.contents, i, childidx));
-        assert old(DisjointSubtrees(node.contents, childidx, (j-1)));
-        assert old(DisjointSubtrees(node.contents, i, (j-1)));
-        assert old(WFShape(node.contents.children[i]));
-        assert old(WFShape(node.contents.children[j-1]));
-      } else if i == childidx    &&      childidx+1 < j {
-        assert old(DisjointSubtrees(node.contents, childidx, (j-1)));
-        assert old(DisjointSubtrees(node.contents, i, (j-1)));
-        assert old(WFShape(node.contents.children[j-1]));
-      } else if i == childidx+1  &&      childidx+1 < j {
-        assert old(DisjointSubtrees(node.contents, childidx, (j-1)));
-        assert old(DisjointSubtrees(node.contents, (i-1), (j-1)));
-        assert old(WFShape(node.contents.children[j-1]));
-      } else {
-        assert old(DisjointSubtrees(node.contents, childidx, (i-1)));
-        assert old(DisjointSubtrees(node.contents, childidx, (j-1)));
-        assert old(DisjointSubtrees(node.contents, (i-1), (j-1)));
-        assert old(WFShape(node.contents.children[i-1]));
-        assert old(WFShape(node.contents.children[j-1]));
-      }
-    }
-
-    assert WFShapeChildren(newchildren, node.repr, node.height);
-  }
-  
-  method SplitChildOfIndex(node: Node, childidx: uint64)
+  method SplitChildOfIndex(linear node: Node, childidx: uint64)
+    returns (linear splitNode: Node)
     requires WF(node)
-    requires node.contents.Index?
+    requires node.Index?
     requires !Full(node)
-    requires 0 <= childidx < node.contents.nchildren
-    requires node.contents.children[childidx] != null
-    requires Full(node.contents.children[childidx]);
-    ensures WFShape(node)
-    ensures node.contents.Index?
-    ensures fresh(node.repr - old(node.repr))
-    ensures node.height == old(node.height)
-    ensures Model.SplitChildOfIndex(old(I(node)), I(node), childidx as int)
-    ensures node.contents.children[childidx] != null
-    ensures node.contents.children[childidx+1] != null
-    ensures !Full(node.contents.children[childidx])
-    ensures !Full(node.contents.children[childidx+1])
-    ensures node.contents.pivots[childidx] in Model.AllKeys(old(I(node)).children[childidx])
-    modifies node, node.contents.pivots, node.contents.children, node.contents.children[childidx]
+    requires 0 <= childidx as nat < |node.children|
+    requires Full(node.children[childidx as nat]);
+    ensures splitNode.Index?
+    ensures Model.SplitChildOfIndex(node, splitNode, childidx as int)
+    ensures WF(splitNode)
+    ensures !Full(splitNode.children[childidx as nat])
+    ensures !Full(splitNode.children[childidx as nat + 1])
+    ensures splitNode.pivots[childidx] in Model.AllKeys(node.children[childidx as nat])
+    ensures Height(splitNode) <= Height(node)
   {
-    assert WFShapeChildren(node.contents.children[..node.contents.nchildren], node.repr, node.height);
-    
-    forall i | 0 <= i < node.contents.nchildren
-      ensures I(node).children[i] == I(node.contents.children[i])
-    {
-      IOfChild(node, i as int);
-    }
-    
-    var right, pivot := SplitNode(node.contents.children[childidx]);
-    Arrays.Insert(node.contents.pivots, node.contents.nchildren-1, pivot, childidx);
-    Arrays.Insert(node.contents.children, node.contents.nchildren, right, childidx + 1);
-    node.contents := node.contents.(nchildren := node.contents.nchildren + 1);
-    node.repr := node.repr + right.repr;
+    linear var Index(pivots, children) := node;
 
-    SplitChildOfIndexPreservesWFShape(node, childidx as int);
-    
-    ghost var ioldnode := old(I(node));
-    ghost var inode := I(node);
-    ghost var iright := I(right);
-    ghost var target := Seq.replace1with2(ioldnode.children, inode.children[childidx], iright, childidx as int);
-    forall i | 0 <= i < |inode.children|
-      ensures inode.children[i] == target[i]
-    {
-      IOfChild(node, i);
-      if i < childidx as int {
-        assert old(DisjointSubtrees(node.contents, i as int, childidx as int));
-      } else if i == childidx as int {
-      } else if i == (childidx + 1) as int {
-      } else {
-        assert old(DisjointSubtrees(node.contents, childidx as int, (i-1) as int));      
-      }
-    }
+    linear var origChild;
+    children, origChild := lseq_take(children, childidx);
 
-    IOfChild(node, childidx as int);
-    IOfChild(node, childidx as int + 1);
+    linear var left, right;
+    var pivot;
+    left, right, pivot := SplitNode(origChild);
+    pivots := InsertSeq(pivots, pivot, childidx);
+    children := lseq_give(children, childidx, left);
+    children := InsertLSeq(children, right, childidx + 1);
+    splitNode := Model.Index(pivots, children);
+    Model.SplitChildOfIndexPreservesWF(node, splitNode, childidx as int);
+
+    // Every new child is shorter than some old child.
+    ghost var wit := seq(|splitNode.children|, i requires 0<=i<|splitNode.children| =>
+      if i <= childidx as nat then i else i-1);
+    SeqMaxCorrespondence(IndexHeights(node), IndexHeights(splitNode), wit);
+    assert Height(splitNode) <= Height(node) by { reveal_Height(); }
   }
 
-  method InsertLeaf(node: Node, key: Key, value: Value) returns (oldvalue: Option<Value>)
+  method InsertLeaf(linear node: Node, key: Key, value: Value)
+    returns (linear n2: Node, oldvalue: Option<Value>)
     requires WF(node)
-    requires node.contents.Leaf?
+    requires node.Leaf?
     requires !Full(node)
-    ensures WFShape(node)
-    ensures node.repr == old(node.repr)
-    ensures I(node) == Model.InsertLeaf(old(I(node)), key, value)
-    ensures Model.WF(I(node))
-    ensures Model.Interpretation(I(node)) == Model.Interpretation(old(I(node)))[key := value]
-    ensures Model.AllKeys(I(node)) == Model.AllKeys(old(I(node))) + {key}
-    ensures oldvalue == MapLookupOption(old(Interpretation(node)), key);
-    modifies node, node.contents.keys, node.contents.values
+    ensures n2 == Model.InsertLeaf(node, key, value)
+    ensures WF(n2)
+    ensures Model.Interpretation(n2) == Model.Interpretation(node)[key := value]
+    ensures Model.AllKeys(n2) == Model.AllKeys(node) + {key}
+    ensures oldvalue == MapLookupOption(Interpretation(node), key);
   {
-    reveal_I();
-    Model.reveal_Interpretation();
-    Model.reveal_AllKeys();
-    var posplus1: uint64 := Model.KeysImpl.ArrayLargestLtePlus1(node.contents.keys, 0, node.contents.nkeys, key);
-    if 1 <= posplus1 && node.contents.keys[posplus1-1] == key {
-      oldvalue := Some(node.contents.values[posplus1-1]);
-      node.contents.values[posplus1-1] := value;
+    linear var Leaf(keys, values) := node;
+    var pos: int64 := Model.KeysImpl.ComputeLargestLteShared(keys, key);
+    if 0 <= pos && seq_get(keys, pos as uint64) == key {
+      oldvalue := Some(seq_get(values, pos as uint64));
+      values := seq_set(values, pos as uint64, value);
     } else {
       oldvalue := None;
-      Arrays.Insert(node.contents.keys, node.contents.nkeys, key, posplus1);
-      Arrays.Insert(node.contents.values, node.contents.nkeys, value, posplus1);
-      node.contents := node.contents.(nkeys := node.contents.nkeys + 1);
+      keys := InsertSeq(keys, key, (pos + 1) as uint64);
+      //assume Model.Keys.IsStrictlySorted(keys); // TODO(robj): I need a lemma call here.
+      values := InsertSeq(values, value, (pos + 1) as uint64);
     }
-    Model.InsertLeafIsCorrect(old(I(node)), key, value);
+    n2 := Model.Leaf(keys, values);
+    Model.InsertLeafIsCorrect(node, key, value);
+    Model.reveal_Interpretation();
   }
-
-  twostate lemma InsertIndexChildNotFullPreservesWFShape(node: Node, childidx: int)
-    requires old(WFShape(node))
-    requires old(node.contents).Index?
-    requires 0 <= childidx < old(node.contents).nchildren as int
-    requires node.contents.Index?
-    requires node.contents.nchildren == old(node.contents).nchildren
-    requires node.contents.children == old(node.contents.children)
-    requires node.contents.pivots == old(node.contents.pivots)
-    requires node.height == old(node.height)
-    requires old(node.contents.children[childidx]) != null
-    requires node.contents.children[childidx] != null
-    requires unchanged(old(node.repr) - ({node} + old(node.contents.children[childidx].repr)))
-    requires forall i :: 0 <= i < childidx ==> node.contents.children[i] == old(node.contents.children[i])
-    requires forall i :: childidx < i < node.contents.nchildren as int ==> node.contents.children[i] == old(node.contents.children[i])
-    requires WFShape(node.contents.children[childidx])
-    requires node.contents.children[childidx].height == old(node.contents.children[childidx].height)
-    requires fresh(node.contents.children[childidx].repr - old(node.contents.children[childidx].repr))
-    requires node.repr == old(node.repr) + node.contents.children[childidx].repr
-    ensures WFShape(node)
+  
+  lemma ChildrenAreShorter(parent: Node, childidx: nat)
+    requires WF(parent)
+    requires parent.Index?
+    requires 0 <= childidx < |parent.children|
+    ensures Height(parent.children[childidx]) < Height(parent)
   {
-    assert old(WFShapeChildren(node.contents.children[..node.contents.nchildren], node.repr, node.height));
-    assert forall i :: 0 <= i < node.contents.nchildren ==> old(WFShape(node.contents.children[i]));
-    
-    forall i | 0 <= i < node.contents.nchildren as int
-      ensures node.contents.children[i] != null
-      ensures node.contents.children[i] in node.repr
-      ensures node.contents.children[i].repr < node.repr
-      ensures node !in node.contents.children[i].repr
-      ensures node.contents.pivots !in node.contents.children[i].repr
-      ensures node.contents.children !in node.contents.children[i].repr
-      ensures node.contents.children[i].height < node.height
-      ensures WFShape(node.contents.children[i])
-    {
-      if i < childidx {
-        assert old(DisjointSubtrees(node.contents, i, childidx));
-      } else if i == childidx {
-      } else {
-        assert old(DisjointSubtrees(node.contents, childidx, i));
-      }
-    }
-    SeqReprSubsetExtensionality(node.contents.children[..node.contents.nchildren], node.repr);
-      
-    forall i, j | 0 <= i < j < node.contents.nchildren as int
-      ensures DisjointReprs(node.contents.children[..node.contents.nchildren], i,j)
-    {
-      assert old(DisjointSubtrees(node.contents, i, j));
-      if                           j <  childidx       {
-        assert old(DisjointSubtrees(node.contents, i, childidx));
-        assert old(DisjointSubtrees(node.contents, j, childidx));
-      } else if                    j == childidx       {
-        assert old(DisjointSubtrees(node.contents, i, childidx));
-      } else if i < childidx     &&      childidx < j {
-        assert old(DisjointSubtrees(node.contents, i, childidx));
-        assert old(DisjointSubtrees(node.contents, childidx, j));
-      } else if i == childidx    &&      childidx < j {
-        assert old(DisjointSubtrees(node.contents, childidx, j));
-      } else {
-        assert old(DisjointSubtrees(node.contents, childidx, i));
-        assert old(DisjointSubtrees(node.contents, childidx, j));
-      }
-    }
+    var child := parent.children[childidx];
+    assert IndexHeights(parent)[childidx] == Height(child); // trigger
+    assert Height(child) in IndexHeights(parent);  // trigger *harder*
+    reveal_Height();
   }
 
-  method InsertIndexChildNotFull(node: Node, childidx: uint64, key: Key, value: Value)
-    returns (oldvalue: Option<Value>)
+  method InsertIndex(linear node: Node, key: Key, value: Value)
+    returns (linear n2: Node, oldvalue: Option<Value>)
     requires WF(node)
-    requires node.contents.Index?
-    requires childidx as int == Model.Keys.LargestLte(node.contents.pivots[..node.contents.nchildren-1], key) + 1
-    requires node.contents.children[childidx] != null
-    requires !Full(node.contents.children[childidx])
-    ensures WFShape(node)
-    ensures fresh(node.repr - old(node.repr))
-    ensures node.height == old(node.height)
-    ensures Model.WF(I(node))
-    ensures Model.Interpretation(I(node)) == Model.Interpretation(old(I(node)))[key := value]
-    ensures Model.AllKeys(I(node)) <= Model.AllKeys(old(I(node))) + {key}
-    ensures oldvalue == MapLookupOption(old(Interpretation(node)), key)
-    modifies node, node.contents.children[childidx], node.contents.children[childidx].repr
-    decreases node.height, 0
-  {
-    assert WFShapeChildren(node.contents.children[..node.contents.nchildren], node.repr, node.height);
-
-    forall i | 0 <= i < node.contents.nchildren
-      ensures I(node.contents.children[i]) == I(node).children[i]
-    {
-      IOfChild(node, i as int);
-    }
-    
-    oldvalue := InsertNode(node.contents.children[childidx], key, value);
-    assert oldvalue == MapLookupOption(old(Interpretation(node)), key) by {
-      reveal_I();
-      Model.reveal_Interpretation();
-      Model.reveal_AllKeys();
-    }
-    node.repr := node.repr + node.contents.children[childidx].repr;
-    
-    InsertIndexChildNotFullPreservesWFShape(node, childidx as int);
-    
-    ghost var oldinode := old(I(node));
-    ghost var inode := I(node);
-    ghost var oldchild := oldinode.children[childidx];
-    ghost var newchild := inode.children[childidx];
-
-    forall i | 0 <= i < childidx as int
-      ensures inode.children[i] == oldinode.children[i]
-    {
-      IOfChild(node, i);
-      assert old(DisjointSubtrees(node.contents, i, childidx as int));
-    }
-    forall i | childidx as int < i < |inode.children|
-      ensures inode.children[i] == oldinode.children[i]
-    {
-      IOfChild(node, i);
-      assert old(DisjointSubtrees(node.contents, childidx as int, i));
-    }
-
-    IOfChild(node, childidx as int);
-    Model.RecursiveInsertIsCorrect(oldinode, key, value, childidx as int, inode, inode.children[childidx]);
-  }
-
-  method InsertIndexSelectAndPrepareChild(node: Node, key: Key) returns (childidx: uint64)
-    requires WF(node)
-    requires node.contents.Index?
+    requires node.Index?
     requires !Full(node)
-    ensures WFShape(node)
-    ensures fresh(node.repr - old(node.repr))
-    ensures node.height == old(node.height)
-    ensures Model.WF(I(node))
-    ensures node.contents.Index?
-    ensures childidx as int == Model.Keys.LargestLte(node.contents.pivots[..node.contents.nchildren-1], key) + 1
-    ensures node.contents.children[childidx] != null
-    ensures !Full(node.contents.children[childidx])
-    ensures Model.Interpretation(I(node)) == Model.Interpretation(old(I(node)))
-    ensures Model.AllKeys(I(node)) == Model.AllKeys(old(I(node)))
-    modifies node, node.repr
+    ensures WF(n2)
+    ensures Model.Interpretation(n2) == Model.Interpretation(node)[key := value]
+    ensures Model.AllKeys(n2) <= Model.AllKeys(node) + {key}  // shouldn't this be ==?
+    ensures oldvalue == MapLookupOption(Interpretation(node), key)
+    decreases Height(node), 1
   {
-    Model.reveal_AllKeys();
-    assert WFShapeChildren(node.contents.children[..node.contents.nchildren], node.repr, node.height);
+    n2 := node;
+    var childidx := Route(n2.pivots, key);
+    if Full(lseq_peek(n2.children, childidx)) {
+      n2 := SplitChildOfIndex(n2, childidx);
 
-    childidx := Model.KeysImpl.ArrayLargestLtePlus1(node.contents.pivots, 0, node.contents.nchildren-1, key);
-    if Full(node.contents.children[childidx]) {
-      ghost var oldpivots := node.contents.pivots[..node.contents.nchildren-1];
-      SplitChildOfIndex(node, childidx);
-      ghost var newpivots := node.contents.pivots[..node.contents.nchildren-1];
-      Model.SplitChildOfIndexPreservesWF(old(I(node)), I(node), childidx as int);
-      Model.SplitChildOfIndexPreservesInterpretation(old(I(node)), I(node), childidx as int);
-      Model.SplitChildOfIndexPreservesAllKeys(old(I(node)), I(node), childidx as int);
+      Model.SplitChildOfIndexPreservesWF(node, n2, childidx as nat);
+      Model.SplitChildOfIndexPreservesInterpretation(node, n2, childidx as nat);
+      Model.SplitChildOfIndexPreservesAllKeys(node, n2, childidx as nat);
+      assert n2.pivots[childidx] in Model.AllKeys(node) by { Model.reveal_AllKeys(); }
 
-      var t: int32 := Model.KeysImpl.cmp(node.contents.pivots[childidx], key);
+      var t: int32 := Model.KeysImpl.cmp(seq_get(n2.pivots, childidx), key);
       if  t <= 0 {
         childidx := childidx + 1;
-        forall i | childidx as int - 1 < i < |newpivots|
-          ensures Model.Keys.lt(key, newpivots[i])
+        forall i | childidx as int - 1 < i < |n2.pivots|
+          ensures Model.Keys.lt(key, n2.pivots[i])
         {
-          assert newpivots[i] == oldpivots[i-1];
+          assert n2.pivots[i] == node.pivots[i-1];
         }
       }
-      Model.Keys.LargestLteIsUnique(node.contents.pivots[..node.contents.nchildren-1], key, childidx as int - 1);
+      Model.Keys.LargestLteIsUnique(n2.pivots, key, childidx as int - 1);
+      assert Interpretation(n2) == Interpretation(node);
     }
-  }
-  
-  method InsertIndex(node: Node, key: Key, value: Value) returns (oldvalue: Option<Value>)
-    requires WF(node)
-    requires node.contents.Index?
-    requires !Full(node)
-    ensures WFShape(node)
-    ensures fresh(node.repr - old(node.repr))
-    ensures node.height == old(node.height)
-    ensures Model.WF(I(node))
-    ensures Model.Interpretation(I(node)) == Model.Interpretation(old(I(node)))[key := value]
-    ensures Model.AllKeys(I(node)) <= Model.AllKeys(old(I(node))) + {key}
-    ensures oldvalue == MapLookupOption(old(Interpretation(node)), key)
-    modifies node, node.repr
-    decreases node.height, 1
-  {
-    var childidx: uint64 := InsertIndexSelectAndPrepareChild(node, key);
-    oldvalue := InsertIndexChildNotFull(node, childidx, key, value);
-  }
-  
-  method InsertNode(node: Node, key: Key, value: Value) returns (oldvalue: Option<Value>)
-    requires WF(node)
-    requires !Full(node)
-    ensures WFShape(node)
-    ensures fresh(node.repr - old(node.repr))
-    ensures node.height == old(node.height)
-    ensures Model.WF(I(node))
-    ensures Model.Interpretation(I(node)) == Model.Interpretation(old(I(node)))[key := value]
-    ensures Model.AllKeys(I(node)) <= Model.AllKeys(old(I(node))) + {key}
-    ensures oldvalue == MapLookupOption(old(Interpretation(node)), key)
-    modifies node, node.repr
-    decreases node.height, 2
-  {
-    if node.contents.Leaf? {
-      oldvalue := InsertLeaf(node, key, value);
+    ghost var preparedNode := n2;
+    assert Height(preparedNode) <= Height(node);
+    assert Interpretation(preparedNode) == Interpretation(node);
+
+    linear var Index(pivots, children) := n2;
+    linear var childNode;
+    // Note(Andrea): In Rust, childNode would be a mutable borrow from
+    // children, and InsertNode would borrow it.
+    children, childNode := lseq_take(children, childidx);
+    ghost var childNodeSnapshot := childNode;
+    assert Height(childNode) < Height(preparedNode) by { ChildrenAreShorter(preparedNode, childidx as nat); }
+    assert Height(childNode) < Height(node);
+    childNode, oldvalue := InsertNode(childNode, key, value);
+    children := lseq_give(children, childidx, childNode);
+    n2 := Model.Index(pivots, children);
+    Model.RecursiveInsertIsCorrect(preparedNode, key, value, childidx as int, n2, n2.children[childidx as int]);
+    if oldvalue.Some? {
+      Model.InterpretationDelegation(preparedNode, key);
     } else {
-      oldvalue := InsertIndex(node, key, value);
+      Model.reveal_Interpretation();
     }
   }
 
-  method Grow(root: Node) returns (newroot: Node)
+  method InsertNode(linear node: Node, key: Key, value: Value)
+    returns (linear n2: Node, oldvalue: Option<Value>)
+    requires WF(node)
+    requires !Full(node)
+    ensures WF(n2)
+    ensures Model.Interpretation(n2) == Model.Interpretation(node)[key := value]
+    ensures Model.AllKeys(n2) <= Model.AllKeys(node) + {key}  // shouldn't this be ==?
+    ensures oldvalue == MapLookupOption(Interpretation(node), key)
+    decreases Height(node), 2
+  {
+    if node.Leaf? {
+      n2, oldvalue := InsertLeaf(node, key, value);
+    } else {
+      n2, oldvalue := InsertIndex(node, key, value);
+    }
+  }
+
+  method Grow(linear root: Node) returns (linear newroot: Node)
     requires WF(root)
     requires Full(root)
-    ensures WFShape(newroot)
-    ensures fresh(newroot.repr - root.repr)
-    ensures newroot.height == root.height + 1
-    ensures I(newroot) == Model.Grow(I(root))
+    ensures WF(newroot)
+    ensures newroot == Model.Grow(root)
     ensures !Full(newroot)
   {
-    newroot := new Node;
-    var newpivots := newArrayFill(MaxChildren()-1, DefaultKey());
-    var newchildren := newArrayFill(MaxChildren(), null);
-    newchildren[0] := root;
-    newroot.contents := Index(1, newpivots, newchildren);
-    newroot.repr := {newroot, newpivots, newchildren} + root.repr;
-    newroot.height := root.height + 1;
-
-    assert WFShapeChildren(newroot.contents.children[..1], newroot.repr, newroot.height) by { reveal_SeqRepr(); }
-    
-    ghost var inewroot := I(newroot);
-    IOfChild(newroot, 0);
-    assert inewroot.children == [ I(root) ];
+    linear var pivots := seq_alloc_init(0, DefaultKey());
+    linear var children := lseq_alloc(1);
+    children := lseq_give(children, 0, root);
+    newroot := Model.Index(pivots, children);
+    assert lseqs(children) == [root]; // trigger
+    ImagineInverse(children);
   }
 
   lemma FullImpliesAllKeysNonEmpty(node: Node)
     requires WF(node)
     requires Full(node)
-    ensures Model.AllKeys(I(node)) != {}
+    ensures Model.AllKeys(node) != {}
   {
-    var inode := I(node);
-    if inode.Leaf? {
-      assert inode.keys[0] in Model.AllKeys(inode) by { Model.reveal_AllKeys(); }
+    if node.Leaf? {
+      assert node.keys[0] in Model.AllKeys(node) by { Model.reveal_AllKeys(); }
     } else {
-      assert inode.pivots[0] in Model.AllKeys(inode) by { Model.reveal_AllKeys(); }
+      assert node.pivots[0] in Model.AllKeys(node) by { Model.reveal_AllKeys(); }
     }
   }
   
-  method Insert(root: Node, key: Key, value: Value) returns (newroot: Node, oldvalue: Option<Value>)
+  method Insert(linear root: Node, key: Key, value: Value)
+    returns (linear newroot: Node, oldvalue: Option<Value>)
     requires WF(root)
     ensures WF(newroot)
-    ensures fresh(newroot.repr - old(root.repr))
-    ensures Interpretation(newroot) == old(Interpretation(root))[key := value]
-    ensures oldvalue == MapLookupOption(old(Interpretation(root)), key)
-    modifies root.repr
+    ensures Interpretation(newroot) == Interpretation(root)[key := value]
+    ensures oldvalue == MapLookupOption(Interpretation(root), key)
   {
     if Full(root) {
       FullImpliesAllKeysNonEmpty(root);
-      Model.GrowPreservesWF(I(root));
+      Model.GrowPreservesWF(root);
       newroot := Grow(root);
-      Model.GrowPreservesInterpretation(I(root));
+      Model.GrowPreservesInterpretation(root);
     } else {
       newroot := root;
     }
-    assert Model.Interpretation(I(newroot)) == Model.Interpretation(old(I(root)));
-    oldvalue := InsertNode(newroot, key, value);
+    assert Model.Interpretation(newroot) == Model.Interpretation(root);
+    newroot, oldvalue := InsertNode(newroot, key, value);
+  }
+
+  method Free(linear node: Node)
+    requires WF(node)
+  {
+    linear match node {
+      case Leaf(keys, values) => {
+        var _ := seq_free(keys);
+        var _ := seq_free(values);
+      }
+      case Index(pivots, children) => {
+        var _ := seq_free(pivots);
+        var i:uint64 := 0;
+        linear var arr := children;
+        while (i < lseq_length_uint64(arr))
+          invariant 0 <= i as int <= |arr|
+          invariant |arr| == |children|
+          invariant forall j | 0 <= j < |arr| :: j in arr <==> j >= i as int
+          invariant forall j | i as int <= j < |arr| :: arr[j] == children[j]
+        {
+          linear var child;
+          arr, child := lseq_take(arr, i);
+          Free(child);
+          i := i + 1;
+        }
+        lseq_free(arr);
+      }
+    }
   }
 }
 
